pass saltLen as an argument

code/experimental/rsa/RSA.fst
@@ -5,6 +5,7 @@ open FStar.Buffer
 open FStar.Int.Cast
 open FStar.All
 open FStar.Mul
+open C.Loops
 
 open Lib
 open Convert
@@ -16,7 +17,6 @@ module U8 = FStar.UInt8
 
 inline_for_extraction let zero_8 = 0uy
 inline_for_extraction let hLen = 32ul
-inline_for_extraction let sLen = 20ul
 
 noeq type rsa_pubkey =
 	| Mk_rsa_pubkey: n:bignum -> e:bignum -> rsa_pubkey
@@ -29,52 +29,48 @@ val get_length_em: (* consider the case when modBits - 1 is divisible by 8 *)
 let get_length_em modBits = bits_to_text modBits
 
 val xordb:
-	b1:uint8_p ->
-	b2:uint8_p{length b2 = length b1} ->
-	len:U32.t{U32.v len <= length b1} -> Stack unit
+	len:U32.t ->
+	b1:lbytes len ->
+	b2:lbytes len{disjoint b1 b2} -> Stack unit
 	(requires (fun h -> live h b1 /\ live h b2))
-	(ensures (fun h0 _ h1 -> live h0 b1 /\ live h0 b2 /\ live h1 b1 /\ modifies_1 b1 h0 h1))
-	(decreases len)
-let rec xordb b1 b2 len =
-	push_frame();
-	if U32.(len >^ 0ul) then
-		let len = U32.(len -^ 1ul) in
-		b1.(len) <- U8.(b1.(len) ^^ b2.(len));
-		xordb b1 b2 len
-	else ();
-	pop_frame()
+	(ensures (fun h0 _ h1 -> live h0 b1 /\ live h0 b2 /\ 
+		live h1 b1 /\ live h1 b2 /\ modifies_1 b1 h0 h1))
+
+let xordb len b1 b2 =
+	C.Loops.in_place_map2 b1 b2 len (fun x y -> U8.(x ^^ y))
 
 val pss_encode:
-	modBits:U32.t{U32.v (get_length_em modBits) >= U32.(v (sLen +^ hLen +^ 2ul))} ->
+	saltLen:U32.t ->
+	modBits:U32.t{U32.v (get_length_em modBits) >= U32.(v (saltLen +^ hLen +^ 2ul))} ->
 	msg:uint8_p -> len:U32.t{U32.v len = length msg} ->
-	salt:uint8_p{length salt = U32.v sLen} ->
+	salt:uint8_p{length salt = U32.v saltLen} ->
 	em:uint8_p{length em = U32.v (get_length_em modBits)} -> Stack unit
 	(requires (fun h -> live h msg /\ live h em /\ live h salt))
 	(ensures (fun h0 _ h1 -> live h0 msg /\ live h0 em /\  live h0 salt /\ live h1 em /\ modifies_1 em h0 h1))
-let pss_encode modBits msg len salt em =
+let pss_encode saltLen modBits msg len salt em =
 	push_frame();
 	let mHash = create zero_8 hLen in
 	hash_sha256 mHash len msg;
 	let emBits = U32.(modBits -^ 1ul) in
 	let emLen = get_length_em modBits in
-	let m1_size = U32.(8ul +^ hLen +^ sLen) in
+	let m1_size = U32.(8ul +^ hLen +^ saltLen) in
 	let m1 = create zero_8 m1_size in
 	(* first 8 elements should be 0x00 *)
 	blit mHash 0ul m1 8ul hLen;
-	blit salt 0ul m1 U32.(8ul +^ hLen) sLen;
+	blit salt 0ul m1 U32.(8ul +^ hLen) saltLen;
 	let m1Hash = create zero_8 hLen in
 	hash_sha256 m1Hash m1_size m1;
 
 	let db_size = U32.(emLen -^ hLen -^ 1ul) in
 	let db = create zero_8 db_size in
-	let ind_1 = U32.(emLen -^ sLen -^ hLen -^ 2ul) in
+	let ind_1 = U32.(emLen -^ saltLen -^ hLen -^ 2ul) in
 	db.(ind_1) <- 1uy;
-	blit salt 0ul db U32.(ind_1 +^ 1ul) sLen;
+	blit salt 0ul db U32.(ind_1 +^ 1ul) saltLen;
 
 	let dbMask = create zero_8 db_size in
 	mgf_sha256 m1Hash db_size dbMask;
 
-	xordb db dbMask db_size;
+	xordb db_size db dbMask;
 	let zeroL = U32.(8ul *^ emLen -^ emBits) in
 	db.(0ul) <- U8.(db.(0ul) &^ (0xffuy >>^ zeroL));
 
@@ -84,16 +80,17 @@ let pss_encode modBits msg len salt em =
 	pop_frame()
 
 val pss_verify:
-	modBits:U32.t{U32.v (get_length_em modBits) >= U32.(v (sLen +^ hLen +^ 2ul))} ->
+	saltLen:U32.t ->
+	modBits:U32.t{U32.v (get_length_em modBits) >= U32.(v (saltLen +^ hLen +^ 2ul))} ->
 	em:uint8_p{length em = U32.v (get_length_em modBits)} ->
 	msg:uint8_p -> len:U32.t{U32.v len = length msg} -> Stack bool
 	(requires (fun h -> live h msg /\ live h em))
 	(ensures (fun h0 _ h1 -> live h0 msg /\ live h0 em /\ live h1 msg /\ live h1 em))
-let pss_verify modBits em msg len =
+let pss_verify saltLen modBits em msg len =
 	push_frame();
 	let emLen = get_length_em modBits in
-	let m1_size = U32.(8ul +^ hLen +^ sLen) in
-	let pad_size = U32.(emLen -^ sLen -^ hLen -^ 1ul) in
+	let m1_size = U32.(8ul +^ hLen +^ saltLen) in
+	let pad_size = U32.(emLen -^ saltLen -^ hLen -^ 1ul) in
 	let db_size = U32.(emLen -^ hLen -^ 1ul) in
 
 	let mHash = create zero_8 hLen in
@@ -111,31 +108,32 @@ let pss_verify modBits em msg len =
 	let tmp = U8.(maskedDB.(0ul) &^ (0xffuy <<^ U32.(8ul -^ zeroL))) in
 	if not (U8.(tmp =^ 0x00uy)) then false else (
 	mgf_sha256 m1Hash db_size dbMask;
-	xordb maskedDB dbMask db_size;
+	xordb db_size maskedDB dbMask;
 	maskedDB.(0ul) <- U8.(maskedDB.(0ul) &^ (0xffuy >>^ zeroL));
 	upd pad2 U32.(pad_size -^ 1ul) 0x01uy;
 
 	let pad = sub maskedDB 0ul pad_size in
 	if not (eqb pad pad2 pad_size) then false else (
-	let salt = sub maskedDB pad_size sLen in
+	let salt = sub maskedDB pad_size saltLen in
 	(* first 8 elements should be 0x00 *)
 	blit mHash 0ul m1 8ul hLen;
-	blit salt 0ul m1 U32.(8ul +^ hLen) sLen;
+	blit salt 0ul m1 U32.(8ul +^ hLen) saltLen;
 	hash_sha256 m1Hash' m1_size m1;
 	eqb m1Hash m1Hash' hLen))) in
 	pop_frame();
 	res
 
 val rsa_sign:
-	modBits:U32.t{U32.v (get_length_em modBits) >= U32.(v (sLen +^ hLen +^ 2ul))} ->
+	saltLen:U32.t ->
+	modBits:U32.t{U32.v (get_length_em modBits) >= U32.(v (saltLen +^ hLen +^ 2ul))} ->
 	skeyBits:U32.t -> msgLen:U32.t ->
 	msg:uint8_p{length msg = U32.v msgLen} ->
 	skey:rsa_privkey ->
-	salt:uint8_p{length salt = U32.v sLen} ->
+	salt:uint8_p{length salt = U32.v saltLen} ->
 	sgnt:uint8_p{length sgnt = U32.v (bits_to_text modBits)} -> Stack unit
 	(requires (fun h -> live h msg /\ live h salt /\ live h sgnt))
 	(ensures (fun h0 _ h1 -> live h0 msg /\ live h0 salt /\ live h0 sgnt /\ live h1 sgnt /\ modifies_1 sgnt h0 h1))
-let rsa_sign modBits skeyBits msgLen msg skey salt sgnt =
+let rsa_sign saltLen modBits skeyBits msgLen msg skey salt sgnt =
 	push_frame();
 	let k = bits_to_text modBits in
 	let d = Mk_rsa_privkey?.d skey in
@@ -144,46 +142,47 @@ let rsa_sign modBits skeyBits msgLen msg skey salt sgnt =
 
 	let emLen = get_length_em modBits in
 	let em = create zero_8 emLen in
-	pss_encode modBits msg msgLen salt em;
+	pss_encode saltLen modBits msg msgLen salt em;
 	let mLen = get_size_nat emLen in
 	let m = create 0uL mLen in
 	text_to_nat emLen em m;
 
 	(* todo: m % n *)
-	let sLen = get_size_nat k in
-	let s = create 0uL sLen in
-    mod_exp modBits mLen skeyBits sLen n m d s;
+	let signLen = get_size_nat k in
+	let s = create 0uL signLen in
+    mod_exp modBits mLen skeyBits signLen n m d s;
 
 	nat_to_text k s sgnt;
 	pop_frame()
 
 val rsa_verify:
-	modBits:U32.t{U32.v (get_length_em modBits) >= U32.(v (sLen +^ hLen +^ 2ul))} ->
+	saltLen:U32.t ->
+	modBits:U32.t{U32.v (get_length_em modBits) >= U32.(v (saltLen +^ hLen +^ 2ul))} ->
 	msgLen:U32.t -> pkeyBits:U32.t ->
 	sgnt:uint8_p{length sgnt = U32.v (bits_to_text modBits)} ->
 	pkey:rsa_pubkey ->
 	msg:uint8_p{length msg = U32.v msgLen} -> Stack bool
 	(requires (fun h -> live h msg /\ live h sgnt))
 	(ensures (fun h0 _ h1 -> live h0 msg /\ live h0 sgnt /\ live h1 msg /\ live h1 sgnt))
-let rsa_verify modBits msgLen pkeyBits sgnt pkey msg =
+let rsa_verify saltLen modBits msgLen pkeyBits sgnt pkey msg =
 	push_frame();
 	let e = Mk_rsa_pubkey?.e pkey in
 	let n = Mk_rsa_pubkey?.n pkey in
 
 	(* the length of the signature in octets *)
 	let k = bits_to_text modBits in
-	let sLen = get_size_nat k in
-	let s = create 0uL sLen in
+	let signLen = get_size_nat k in
+	let s = create 0uL signLen in
 	text_to_nat k sgnt s;
 
 	(* todo: s % n *)
 	let emLen = get_length_em modBits in
 	let mLen = get_size_nat emLen in
 	let m = create 0uL mLen in
-	mod_exp modBits sLen pkeyBits mLen n s e m;
+	mod_exp modBits signLen pkeyBits mLen n s e m;
 
 	let em = create zero_8 emLen in
 	nat_to_text emLen m em;
-	let res = pss_verify modBits em msg msgLen in
+	let res = pss_verify saltLen modBits em msg msgLen in
 	pop_frame();
 	res
